\chapter{ODE and Boundary Problems}
\lecture{20}{9 Apr 2025 10:10}{}
\section{Initial Value Problems}
Consider an initial value problem we thus want to solve for 
\[
    \frac{\mathrm{d}y}{\mathrm{d}t} = f(t,y) , \quad a \leq  t \leq  b
\]
\[
    y(a) = y_a
\]
\begin{definition}
    A function \(f(t,y)\) is Lipschitz continuous with Lipschitz constant \(L\) 
    in the variable \(y\)  if 
    \[
        \vert f(t,y_1) - f(t,y_2)\vert \leq  L \vert y_1 - y_2 \vert. 
        \quad \forall (t, y_1) , (t,y_2) \in \text{Dom}(f)  
    \]
\end{definition}
\begin{eg}
Consider 
\[
    f(t,y) = t \vert y \vert 
\]
\[
    D = \left\{ (t,y) | 1 \leq  t \leq  2, -3 \leq  y \leq  4 \right\} 
\]
We can check this that 
\[
    \vert ty_1 - ty_2 \vert \leq  L \vert y_1 - y_2 \vert 
\]
Therefore we must have that \( L =  2\) 
\end{eg}

\begin{theorem}
    Let \(\mathcal{D} = \left\{ (t,y) | a \leq  t \leq  b , - \infty  < y < \infty  \right\}
     \) and \(f\) is Lipschitz continuous. Then the IVP must have a unique solution. 
\end{theorem}
\begin{eg}
Consider 
\[
    y^{\prime} (t) = 1 + t \sin  (ty), \quad 0 \leq  t \leq  2
\]
\[
    y(0) = 0
\]
It must be that my MVT
\[
    \frac{f(t, y_2) - f(t, y_1)}{y_2 - y_1 } = \frac{\partial f}{\partial y} (t, \zeta)
\]
\[
    \vert f(t,y_2) - f(t,y_1) \vert = t^{2}  \cos (t \zeta) \vert y_2 - y_1 \vert \leq  4 \vert y_2 - y_1 \vert 
\]
Thus \(L = 4\) 
\end{eg}
\section{Forward Euler}
\begin{definition}
    Time grid is the time instances covered in \(\left[ a,b \right] \)
    \[
        a = t_0 < t_1 < \dots  < t_{N-1} < t_N = b 
    \] 
    Therefore 
    \[
        t_i = a + ih, \quad h = \frac{b-a}{N}
    \]
\end{definition}
With this we can construct the derivatives at each point to calculate the values of \(y\) 
\begin{definition}
    Forward Euler's uses a forward finite difference scheme
    \[
        \frac{\mathrm{d}y}{\mathrm{d}t} (t_i) \approx \frac{y(t_{i+1} ) - y(t_i)}{h}
    \]
    Rewriting we must have taht 
    \[
        y(t_{i+1} ) = y(t_i) + h f(t_i, y(t_i)), \quad i = 0,1, \dots , N-1
    \]
\end{definition}
This makes any problem trivial to find future values given an IVP:


\begin{algorithm}[H]
    \caption{Forward Euler Method}
    \KwIn{$a, b, y_0, N, f$}
    \KwOut{$y$}
    \BlankLine
    $h \gets \frac{b-a}{N}$\;
    $y[0:N] \gets 0$; $y[0] \gets y_0$\;
    \For{$j = 0$ \KwTo $N-1$}{
        $t \gets a + j \cdot h$\;
        $y[j+1] \gets y[j] + h \cdot f(t, y[j])$\;
    }
    \Return{$y$}\;
    \end{algorithm}

\section{Backward Euler Method}
\begin{definition}
    Consider the backward finite difference where
\[
    \frac{\mathrm{d}y}{\mathrm{d}t} (t_i) \approx \frac{y(t_i) - y(t_{i-1})}{h}
\]
\[
    y(t_i) - hf(t_i, y(t_i)) = y(t_{i-1} )
\]
\end{definition}
We can then backwards solve for the next values. 

\begin{algorithm}
    \caption{Backward Euler Method}
    \KwIn{\(a, b, y_0, N , f\) }
    \(h = \frac{b-a}{N}\)\;
    \For{\(j =1 \)  \KwTo \(N\)}{
        \(t = a + i \cdot  h\)\;
        \(y[j] = \text{solve} \left(  g(x,t) , y[i-1] \right) \)  \;
    }
    \Return{\(y\)}\;
\end{algorithm}

\section{Elementary Error Analysis}
Choose \(\left\{ Y \right\}_{i=0}^N \) to be the numerical solution of an IVP, then we have
\[
    \frac{Y_{i+1} - Y_i}{h} = f(t_i, Y_I)
\] 
\begin{definition}
    Trucation Error is defined to be the residual we get from truncating our solution when we replace \(Y_i\) by \(y(t_i)\) 
    \[
        \tau_{i+1}(h,i,y) = \frac{y(t_{i+1} - y(t_i))}{h} - f(t_i, y(t_i)) 
    \]
\end{definition}

\begin{definition}
    The order of accuracy is s.t. for \( C > 0\) 
    \[
        \vert \tau_{i+1}  \vert \leq C h^p, \quad t \in \left[ 0, T \right] 
    \]
\end{definition}
Consider forward euler using a taylor expansion we will get 
\[
    y(t) = y(t_i) + (t-t_i ) y^{\prime} (t_i) + 
    \frac{y^{\prime\prime} }{2} (t-t_i)^{2}  + \mathcal{O}  ((t-t_i)^{3} )
\]
Plugging into the forward euler method for both points 
\[
    \tau_i (h,i,y) = \frac{y(t_{i+1} - y(t_i) )}{h} - f(t_i, y(t_i))
\]
\[
    = \frac{y(t_{i+1} - y(t_i) )}{h} - y^{\prime} (t_i)
\]
\[
    = \frac{y^{\prime\prime} (t_i) }{2} h +  \mathcal{O}  (h^{2}  )
\]

\section{Higher Order Methods}
Consider IVP of ODEs with taylor expansions with \(y\) that are sufficiently regular. 
We will directly consider the nth order scheme given in taylor's method where 
\[
    Y_{i+1} = Y_i + h T^{(n)} (t_I, Y_i), \quad Y_0 = y_a
\]
\[
    T^{(n)} (t_i, Y_i) = f(t_i, Y_i) + \frac{h}{2} f^{\prime} (t_i,Y_i) + \dots  + 
    \frac{h^{n-1} }{n!} f^{(n-1)}(t_i. Y_I)
\]