\lecture{13}{11 Mar 2025}{10:10}
\section{Lagrange Interpolation Proof}
\begin{proof}
    The Lagnrange polynomial \(L_{nk} (x) \) is given as 
    \[
        L_{nk}(x) = 
        \prod_{i=0, i\neq  k}^n \frac{x-x_i}{x_k - x_i} 
    \]
    If \(L_{nk} (x_j) = \delta_{kj} \) then if \(k=j\) the whole expression cancels to be one. And \(0\) if otherwise. 
    Let us now show that 
    \[
        P(x_j) = \sum_{k=0}^{n} f(x_k)L_{nk} (x_j) = f(x_j), \quad 0 \leq  j \leq n
    \]
\end{proof}